Organizing Imp2AsmCorrectness

tutorial/Imp2AsmCorrectness.v
@@ -43,6 +43,10 @@ Local Open Scope cat.
 
 (* end hide *)
 
+(* ================================================================= *)
+(** ** Hiding mangling of variables. *)
+
+(** [varOf] and [gen_tmp] are injective. *)
 Section GEN_TMP.
 
   Lemma gen_tmp_inj: forall n m, m <> n -> gen_tmp m <> gen_tmp n.
@@ -61,18 +65,47 @@ End GEN_TMP.
 Opaque gen_tmp.
 Opaque varOf.
 
+(* ================================================================= *)
+(** ** Simulation relations *)
+
+(** The compiler is proved correct by constructing a (itree) bisimulation between
+    the source program and its compilee.
+    As is traditional, we define to this end a simulation relation [Renv]. Since the
+    bisimulation will take place after handling of the local environment, [Renv]
+    relates two [alist var value] environments.
+ *)
+
 Section Simulation_Relation.
 
-  Variable E: Type -> Type.
-  Context {HasLocals: Locals -< E} {HasMemory: Memory -< E}.
+  (** ** Definition of the simulation relations *)
 
+  (** Relates a source variable to its mangled counterpart in _Asm_. *)
   Variant Rvar : var -> var -> Prop :=
   | Rvar_var v : Rvar (varOf v) v.
 
+  (** The simulation relation for evaluation of statements.
+      The relation relates two environments of type [alist var value].
+      The source and target environments exactly agree on user variables.
+   *)
   Definition Renv (g_asm g_imp : alist var value) : Prop :=
     forall k_asm k_imp, Rvar k_asm k_imp ->
                    forall v, alist_In k_imp g_imp v <-> alist_In k_asm g_asm v.
 
+ (** The simulation relation for evaluation of expressions.
+     The relation also relates two environments of type [alist var value],
+     but additionally the returned value at the _Imp_ level. The _Asm_
+     side does not carry a [value], but a [unit], since its denotation
+     does not return any [value].
+     The [sim_rel] relation is parameterized by the state of the [asm] environment
+     before the step, and the name of the variable used to store
+     the result.
+     It enforces three conditions:
+     - [Renv] on the environments, ensuring that evaluation of expressions
+     does not corrupt user variables;
+     - Agreement on the computed value, i.e. the returned value [v] is stored at
+     the assembly level in the expected temporary;
+     - The "stack" of temporaries used to compute intermediate results is left untouched.
+  *) 
   Definition sim_rel g_asm n: alist var value * unit -> alist var value * value -> Prop :=
     fun '(g_asm', _) '(g_imp',v) =>
       Renv g_asm' g_imp' /\            (* we don't corrupt any of the imp variables *)
@@ -80,6 +113,10 @@ Section Simulation_Relation.
       (forall m, m < n -> forall v,              (* we don't mess with anything on the "stack" *)
             alist_In (gen_tmp m) g_asm v <-> alist_In (gen_tmp m) g_asm' v).
 
+
+  (** ** Facts on the simulation relations *)
+
+  (** [Renv] is stable by updates to temporaries. *)
   Lemma Renv_add: forall g_asm g_imp n v,
       Renv g_asm g_imp -> Renv (alist_add (gen_tmp n) v g_asm) g_imp.
   Proof.
@@ -91,6 +128,7 @@ Section Simulation_Relation.
     apply In_add_ineq_iff; auto.
   Qed.
 
+  (** [Renv] entails agreement of lookup of user variables. *)
   Lemma Renv_find:
     forall g_asm g_imp x,
       Renv g_asm g_imp ->
@@ -106,6 +144,7 @@ Section Simulation_Relation.
       rewrite LUR in LUL; inv LUL.
   Qed.      
 
+  (** [sim_rel] can be initialized from [Renv]. *)
   Lemma sim_rel_add: forall g_asm g_imp n v,
       Renv g_asm g_imp ->
       sim_rel g_asm n (alist_add (gen_tmp n) v g_asm, tt) (g_imp, v).
@@ -118,6 +157,7 @@ Section Simulation_Relation.
       apply In_add_ineq_iff, gen_tmp_inj; lia.
   Qed.
 
+  (** [Renv] can be recovered from [sim_rel]. *)
   Lemma sim_rel_Renv: forall g_asm n s1 v1 s2 v2,
       sim_rel g_asm n (s1,v1) (s2,v2) -> Renv s1 s2.
   Proof.
@@ -132,6 +172,8 @@ Section Simulation_Relation.
     intros ? ? ? ? ? [_ [H _]]; exact H. 
   Qed.
 
+  (** [sim_rel] entails agreement of lookups in the "stack" between its argument
+      and the current Asm environement *)
   Lemma sim_rel_find_tmp_lt_n:
     forall g_asm n m g_asm' g_imp' v,
       m < n ->
@@ -150,15 +192,16 @@ Section Simulation_Relation.
     rewrite EQ' in EQ; easy.
   Qed.
 
+  (** [Renv] is preserved by assignment.
+   *)
   Lemma Renv_write_local:
-    forall (x : Imp.var) (a a0 : alist var value) (v : Imp.value),
-      Renv a a0 -> Renv (alist_add (varOf x) v a) (alist_add x v a0).
+    forall (k : Imp.var) (g_asm g_imp : alist var value) v,
+      Renv g_asm g_imp ->
+      Renv (alist_add (varOf k) v g_asm) (alist_add k v g_imp).
   Proof.
-    intros k m m' v.
-    repeat intro.
-    red in H.
-    specialize (H k_asm k_imp H0 v0).
-    inv H0.
+    intros k m m' v HRel k_asm k_imp Hk v'.
+    specialize (HRel _ _ Hk v').
+    inv Hk.
     unfold alist_add, alist_In; simpl.
     do 2 flatten_goal;
       repeat match goal with
@@ -173,18 +216,43 @@ Section Simulation_Relation.
 
 End Simulation_Relation.
 
-Section Correctness.
+(* ================================================================= *)
+(** ** Bisimulation *)
+
+(** We now make precise the bisimulation established to show the correctness
+    of the compiler.
+    Naturally, we cannot establish a _strong bisimulation_ between the source
+    program and the target program: the [asm] counterpart performs "more
+    steps" when evaluating expressions.
+    The appropriate notion is of course the _equivalence up to tau_. However,
+    the [itree] structures put in evidence a very naturaly hierarchy of notions
+    of correctness.
+    Since the [asm] programs performs more manipulations of its local
+    environment, we cannot hope to relate the trees containing [Locals] events,
+    we first need to interpret them.
+    However, since it does not introduce any manipulation of the heap, we
+    interestingly can prove the result without interpreting the [Memory] events.
+    Of course this example is rather contrieved, owing to the simplicity of the
+    compiler. Nonetheless, it makes a lot of sense when considering optimization:
+    one can see the handling of events are bits of the memory model, and 
+    therefore have a framework to prove some optimization correct with respect
+    to any memory model, i.e. before handling, while other with respect to
+    concrete memory model, i.e. after handling.
+ *)
+
+Section Eq_Locals.
 
   Context {E': Type -> Type}.
-  Context {HasMemory: Memory -< E'}.
-  Context {HasExit: Exit -< E'}.
   Notation E := (Locals +' E').
 
+  (** [interp_locals] handle [Locals] into the [envE] effects, and then
+      run these effects into the state monad. *)
   Definition interp_locals {R: Type} (t: itree E R) (s: alist var value)
     : itree E' (alist var value * R) :=
     run_env _ (interp (bimap evalLocals (id_ _)) _ t) s.
 
-  Instance eutt_interp_locals {R}:
+  (** This interpreter is compatible with the equivalence-up-to-tau. *)
+  Global Instance eutt_interp_locals {R}:
     Proper (@eutt E R R eq ==> eq ==> @eutt E' (prod (alist var value) R) (prod _ R) eq)
            interp_locals.
   Proof.
@@ -195,6 +263,7 @@ Section Correctness.
     rewrite H; reflexivity.
   Qed.
 
+  (** [interp_locals] commutes with [bind]. *)
   Lemma interp_locals_bind: forall {R S} (t: itree E R) (k: R -> itree _ S) (s: alist var value),
       @eutt E' _ _ eq
             (interp_locals (ITree.bind t k) s)
@@ -208,16 +277,28 @@ Section Correctness.
     reflexivity.
   Qed.
 
+  (** Definition of our bisimulation relation.
+      As previously explained, it relates up-to-tau two [itree]s after having
+      interpreted their [Locals] event.
+      We additionally bake into it a simulation relation taken in parameter:
+      - Local events are interpreted from related states.
+      - Returned values must contain related states, as well as computed datas
+      related by another relation [RR] taken in parameter.
+      In our case, we specialize [RR] to equality since both trees return [unit],
+      and [Renv_] to [Renv].
+   *)
+  (* YZ TODO: sim_rel shoudl be expressed in terms of eq_locals? *)
   Definition eq_locals {R1 R2} (RR : R1 -> R2 -> Prop)
              (Renv_ : _ -> _ -> Prop)
-             t1 t2 :=
+             (t1: itree E R1) (t2: itree E R2): Prop :=
     forall g1 g2,
       Renv_ g1 g2 ->
       eutt (fun a (b : alist var value * R2) => Renv_ (fst a) (fst b) /\ RR (snd a) (snd b))
            (interp_locals t1 g1)
            (interp_locals t2 g2).
 
-  Instance eutt_eq_locals (Renv_ : _ -> _ -> Prop) {R} RR :
+  (** [eq_locals] is compatible with [eutt]. *)
+  Global Instance eutt_eq_locals (Renv_ : _ -> _ -> Prop) {R} RR :
     Proper (eutt eq ==> eutt eq ==> iff) (@eq_locals R R RR Renv_).
   Proof.
     repeat intro.
@@ -226,6 +307,7 @@ Section Correctness.
     - rewrite H, H0; auto.
   Qed.
 
+  (** [eq_locals] commutes with [bind]  *)
   Definition eq_locals_bind_gen (Renv_ : _ -> _ -> Prop)
              {R1 R2 S1 S2} (RR : R1 -> R2 -> Prop)
              (RS : S1 -> S2 -> Prop) :
@@ -242,6 +324,7 @@ Section Correctness.
     intros. eapply H0; destruct H2; auto.
   Qed.
 
+  (** [eq_locals] is compatible with [loop]. *)
   Lemma eq_locals_loop {A B C} x (t1 t2 : C + A -> itree E (C + B)) :
     (forall l, eq_locals eq Renv (t1 l) (t2 l)) ->
     eq_locals eq Renv (loop t1 x) (loop t2 x).
@@ -251,6 +334,138 @@ Section Correctness.
     rewrite 2 interp_loop.
     eapply interp_state_loop; auto.
   Qed.
+
+End Eq_Locals.
+
+(* ================================================================= *)
+(** ** Linking *)
+
+(** We first show that our "high level" [asm] combinators are correct.
+    These proofs are mostly independent from the compiler, and therefore
+    fairly reusable.
+    Once again, these notion of correctness are expressed as equations
+    commuting the denotation with the combinator.
+ *)
+
+Section Linking.
+
+  Context {E': Type -> Type}.
+  Context {HasMemory: Memory -< E'}.
+  Context {HasExit: Exit -< E'}.
+  Notation E := (Locals +' E').
+
+  (** [seq_asm] is denoted as the (horizontal) composition of denotations. *)
+  Lemma seq_asm_correct {A B C} (ab : asm A B) (bc : asm B C) :
+      denote_asm (seq_asm ab bc)
+    ⩯ denote_asm ab >>> denote_asm bc.
+  Proof.
+    unfold seq_asm. 
+    rewrite link_asm_correct, relabel_asm_correct, app_asm_correct.
+    rewrite <- lift_ktree_id, cat_assoc.
+    rewrite cat_id_r.
+    rewrite sym_ktree_unfold.
+    apply cat_from_loop.
+    all: typeclasses eauto.
+  Qed.
+
+  (** [if_asm] is denoted as the ktree first denoting the branching condition,
+      then looking-up the appropriate variable and following with either denotation. *)
+  Lemma if_asm_correct {A} (e : list instr) (tp fp : asm unit A) :
+      denote_asm (if_asm e tp fp)
+    ⩯ ((fun _ =>
+         denote_list e ;;
+         v <- lift (GetVar tmp_if) ;;
+         if v : value then denote_asm fp tt else denote_asm tp tt) : ktree _ _ _).
+  Proof.
+    unfold if_asm.
+    rewrite seq_asm_correct.
+    unfold cond_asm.
+    rewrite raw_asm_block_correct_lifted.
+    intros [].
+    unfold CategoryOps.cat, Cat_ktree, ITree.cat; simpl.
+    rewrite after_correct.
+    simpl.
+    repeat setoid_rewrite bind_bind.
+    apply eutt_bind; try reflexivity. intros [].
+    apply eutt_bind; try reflexivity. intros [].
+    - rewrite bind_ret_.
+      rewrite (relabel_asm_correct _ _ _ (inr tt)).
+      unfold CategoryOps.cat, Cat_ktree, ITree.cat; simpl.
+      rewrite bind_bind.
+      unfold lift_ktree; rewrite bind_ret_.
+      setoid_rewrite (app_asm_correct tp fp (inr tt)).
+      setoid_rewrite bind_bind.
+      rewrite <- (bind_ret2 (denote_asm fp tt)) at 2.
+      eapply eutt_bind; try reflexivity. intros ?.
+      unfold inr_, Inr_ktree, lift_ktree; rewrite bind_ret_; reflexivity.
+    - rewrite bind_ret_.
+      rewrite (relabel_asm_correct _ _ _ (inl tt)).
+      unfold CategoryOps.cat, Cat_ktree, ITree.cat; simpl.
+      rewrite bind_bind.
+      unfold lift_ktree; rewrite bind_ret_.
+      setoid_rewrite (app_asm_correct tp fp (inl tt)).
+      setoid_rewrite bind_bind.
+      rewrite <- (bind_ret2 (denote_asm tp tt)) at 2.
+      eapply eutt_bind; try reflexivity. intros ?.
+      unfold inl_, Inl_ktree, lift_ktree;
+        rewrite bind_ret_; reflexivity.
+  Qed.
+
+  (** [while_asm] is denoted as the loop of the body with two entry point, the exit
+      of the loop, and the body in which we have the same structure as for the conditional *)
+   Lemma while_asm_correct (e : list instr) (p : asm unit unit) :
+      denote_asm (while_asm e p)
+    ⩯ loop (fun l : unit + unit =>
+         match l with
+         | inl tt =>
+           denote_list e ;;
+           v <- ITree.lift (inl1 (GetVar tmp_if)) ;;
+           if v : value then
+             Ret (inr tt)
+           else
+             (denote_asm p tt;; Ret (inl tt))
+         | inr tt => Ret (inl tt)
+         end).
+  Proof.
+    unfold while_asm.
+    rewrite link_asm_correct.
+    apply eq_ktree_loop.
+    rewrite relabel_asm_correct.
+    rewrite <- lift_ktree_id, cat_id_l.
+    rewrite app_asm_correct.
+    rewrite if_asm_correct.
+    all: try typeclasses eauto.
+    intros [[] | []].
+    - unfold ITree.cat. 
+      simpl; setoid_rewrite bind_bind.
+      rewrite bind_bind.
+      apply eutt_bind; try reflexivity. intros [].
+      rewrite bind_bind.
+      apply eutt_bind; try reflexivity. intros [].
+      + rewrite (pure_asm_correct _ tt).
+        unfold inl_, Inl_ktree, lift_ktree.
+        repeat rewrite bind_ret_.
+        reflexivity.
+      + rewrite (relabel_asm_correct _ _ _  tt).
+        unfold CategoryOps.cat, Cat_ktree, ITree.cat.
+        simpl; repeat setoid_rewrite bind_bind.
+        unfold inl_, Inl_ktree, lift_ktree; rewrite bind_ret_.
+        apply eutt_bind; try reflexivity. intros [].
+        repeat rewrite bind_ret_; reflexivity.
+    - rewrite itree_eta; cbn; reflexivity.
+  Qed.
+
+End Linking.
+
+(* ================================================================= *)
+(** ** Correctness *)
+
+Section Correctness.
+
+  Context {E': Type -> Type}.
+  Context {HasMemory: Memory -< E'}.
+  Context {HasExit: Exit -< E'}.
+  Notation E := (Locals +' E').
 
   Ltac force_left :=
     match goal with
@@ -264,9 +479,6 @@ Section Correctness.
 
   Ltac untau_left := force_left; rewrite tau_eutt.
   Ltac untau_right := force_right; rewrite tau_eutt.
-
-
-  Notation "(% x )" := (gen_tmp x) (at level 1).
 
   Lemma compile_expr_correct : forall e g_imp g_asm n,
       Renv g_asm g_imp ->
@@ -302,7 +514,7 @@ Section Correctness.
         apply eutt_ret.
         {
           generalize HSIM; intros LU; apply sim_rel_find_tmp_n in LU.
-          unfold alist_In in LU; erewrite sim_rel_find_tmp_lt_n in LU; eauto; fold (alist_In (%n) g_asm'' v) in LU.
+          unfold alist_In in LU; erewrite sim_rel_find_tmp_lt_n in LU; eauto; fold (alist_In (gen_tmp n) g_asm'' v) in LU.
           generalize HSIM'; intros LU'; apply sim_rel_find_tmp_n in LU'.
           rewrite LU,LU'.
           split; [| split].
@@ -338,7 +550,7 @@ Section Correctness.
         apply eutt_ret.
         {
           generalize HSIM; intros LU; apply sim_rel_find_tmp_n in LU.
-          unfold alist_In in LU; erewrite sim_rel_find_tmp_lt_n in LU; eauto; fold (alist_In (%n) g_asm'' v) in LU.
+          unfold alist_In in LU; erewrite sim_rel_find_tmp_lt_n in LU; eauto; fold (alist_In (gen_tmp n) g_asm'' v) in LU.
           generalize HSIM'; intros LU'; apply sim_rel_find_tmp_n in LU'.
           rewrite LU,LU'.
           split; [| split].
@@ -374,7 +586,7 @@ Section Correctness.
         apply eutt_ret.
         {
           generalize HSIM; intros LU; apply sim_rel_find_tmp_n in LU.
-          unfold alist_In in LU; erewrite sim_rel_find_tmp_lt_n in LU; eauto; fold (alist_In (%n) g_asm'' v) in LU.
+          unfold alist_In in LU; erewrite sim_rel_find_tmp_lt_n in LU; eauto; fold (alist_In (gen_tmp n) g_asm'' v) in LU.
           generalize HSIM'; intros LU'; apply sim_rel_find_tmp_n in LU'.
           rewrite LU,LU'.
           split; [| split].
@@ -419,106 +631,6 @@ Section Correctness.
     eapply Renv_write_local; eauto.
   Qed.
 
-  Lemma seq_asm_correct {A B C} (ab : asm A B) (bc : asm B C) :
-      denote_asm (seq_asm ab bc)
-    ⩯ denote_asm ab >>> denote_asm bc.
-  Proof.
-    unfold seq_asm. 
-    rewrite link_asm_correct, relabel_asm_correct, app_asm_correct.
-    rewrite <- lift_ktree_id, cat_assoc.
-    rewrite cat_id_r.
-    rewrite sym_ktree_unfold.
-    apply cat_from_loop.
-    all: typeclasses eauto.
-  Qed.
-
-  Lemma if_asm_correct {A} (e : list instr) (tp fp : asm unit A) :
-      denote_asm (if_asm e tp fp)
-    ⩯ ((fun _ =>
-         denote_list e ;;
-                     v <- lift (GetVar tmp_if) ;;
-                     if v : value then denote_asm fp tt else denote_asm tp tt) : ktree _ _ _).
-  Proof.
-    unfold if_asm.
-    rewrite seq_asm_correct.
-    unfold cond_asm.
-    rewrite raw_asm_block_correct_lifted.
-    intros [].
-    unfold CategoryOps.cat, Cat_ktree, ITree.cat; simpl.
-    rewrite after_correct.
-    simpl.
-    repeat setoid_rewrite bind_bind.
-    apply eutt_bind; try reflexivity. intros [].
-    apply eutt_bind; try reflexivity. intros [].
-    - rewrite bind_ret_.
-      rewrite (relabel_asm_correct _ _ _ (inr tt)).
-      unfold CategoryOps.cat, Cat_ktree, ITree.cat; simpl.
-      rewrite bind_bind.
-      unfold lift_ktree; rewrite bind_ret_.
-      setoid_rewrite (app_asm_correct tp fp (inr tt)).
-      setoid_rewrite bind_bind.
-      rewrite <- (bind_ret2 (denote_asm fp tt)) at 2.
-      eapply eutt_bind; try reflexivity. intros ?.
-      unfold inr_, Inr_ktree, lift_ktree; rewrite bind_ret_; reflexivity.
-    - rewrite bind_ret_.
-      rewrite (relabel_asm_correct _ _ _ (inl tt)).
-      unfold CategoryOps.cat, Cat_ktree, ITree.cat; simpl.
-      rewrite bind_bind.
-      unfold lift_ktree; rewrite bind_ret_.
-      setoid_rewrite (app_asm_correct tp fp (inl tt)).
-      setoid_rewrite bind_bind.
-      rewrite <- (bind_ret2 (denote_asm tp tt)) at 2.
-      eapply eutt_bind; try reflexivity. intros ?.
-      unfold inl_, Inl_ktree, lift_ktree;
-        rewrite bind_ret_; reflexivity.
-  Qed.
-
-  Lemma while_asm_correct (e : list instr) (p : asm unit unit) :
-      denote_asm (while_asm e p)
-    ⩯ loop (fun l : unit + unit =>
-         match l with
-         | inl tt =>
-           denote_list e ;;
-           v <- ITree.lift (inl1 (GetVar tmp_if)) ;;
-           if v : value then
-             Ret (inr tt)
-           else
-             (denote_asm p tt;; Ret (inl tt))
-         | inr tt => Ret (inl tt)
-         end).
-  Proof.
-    unfold while_asm.
-    rewrite link_asm_correct.
-    (* TODO: this is a hack it should just be
-     apply eq_ktree_loop. *)
-    match goal with
-    | [ |- _ (loop ?x) (loop ?y) ] => apply (eq_ktree_loop x y)
-    end.
-    rewrite relabel_asm_correct.
-    rewrite <- lift_ktree_id, cat_id_l.
-    rewrite app_asm_correct.
-    rewrite if_asm_correct.
-    all: try typeclasses eauto.
-    intros [[] | []].
-    - unfold ITree.cat. 
-      simpl; setoid_rewrite bind_bind.
-      rewrite bind_bind.
-      apply eutt_bind; try reflexivity. intros [].
-      rewrite bind_bind.
-      apply eutt_bind; try reflexivity. intros [].
-      + rewrite (pure_asm_correct _ tt).
-        unfold inl_, Inl_ktree, lift_ktree.
-        repeat rewrite bind_ret_.
-        reflexivity.
-      + rewrite (relabel_asm_correct _ _ _  tt).
-        unfold CategoryOps.cat, Cat_ktree, ITree.cat.
-        simpl; repeat setoid_rewrite bind_bind.
-        unfold inl_, Inl_ktree, lift_ktree; rewrite bind_ret_.
-        apply eutt_bind; try reflexivity. intros [].
-        repeat rewrite bind_ret_; reflexivity.
-    - rewrite itree_eta; cbn; reflexivity.
-  Qed.
-
   Lemma while_is_loop {E} (body : itree E bool) :
     while body
           ≈ loop (fun l : unit + unit =>
@@ -549,7 +661,7 @@ Section Correctness.
   Lemma sim_rel_get_tmp0:
     forall g_asm0 g_asm g_imp v,
       sim_rel g_asm0 0 (g_asm,tt) (g_imp,v) ->
-      interp_locals (lift (GetVar (%0))) g_asm ≈ Ret (g_asm,v).
+      interp_locals (E' := E') (lift (GetVar (gen_tmp 0))) g_asm ≈ Ret (g_asm,v).
   Proof.
     intros.
     destruct H as [_ [eq _]].
@@ -576,7 +688,7 @@ Section Correctness.
     reflexivity.
   Qed.
 
-  Lemma compile_correct (s : stmt) :
+  Theorem compile_correct (s : stmt) :
     eq_locals eq Renv
               (denote_asm (compile s) tt)
               (denoteStmt s).
